theories/Core/ITreeMonad.v
@@ -22,16 +22,8 @@ Qed.
 Instance MonadLawsE_ITree {E} : MonadLawsE (itree E).
 Proof.
   constructor.
-  - intros a b f x.
-    unfold Monad.bind, Monad.ret, Monad_itree.
-    unfold eq1, Eq1_ITree. rewrite bind_ret_l. reflexivity.
-  - intros a x.    unfold Monad.bind, Monad.ret, Monad_itree.
-    unfold eq1, Eq1_ITree. rewrite bind_ret_r. reflexivity.
-  - intros a b c x f g. unfold Monad.bind, Monad.ret, Monad_itree.
-    unfold eq1, Eq1_ITree. rewrite bind_bind. reflexivity.
-  - unfold Monad.bind, Monad_itree.
-    intros.
-    repeat red.
-    intros.
-    apply eqit_bind; auto.
+  - intros; unfold eq1, Eq1_ITree. apply eq_sub_eutt, bind_ret_l.
+  - intros; unfold eq1, Eq1_ITree. apply eq_sub_eutt, bind_ret_r.
+  - intros; unfold eq1, Eq1_ITree. apply eq_sub_eutt, bind_bind.
+  - intros; apply eqit_bind.
 Qed.
