theories/Events/StateFacts.v
@@ -26,9 +26,9 @@ From ITree Require Import
      Events.State.
 
 Import ITree.Basics.Basics.Monads.
-Import ITreeNotations.
+Import MonadNotation.
 
-Open Scope itree_scope.
+Local Open Scope monad_scope.
 
 Import Monads.
 (* end hide *)
@@ -54,7 +54,7 @@ Proof.
   - rewrite 2 bind_ret_l. reflexivity.
   - rewrite 2 bind_ret_l.
     reflexivity.
-  - rewrite bind_map, bind_bind; cbn. setoid_rewrite bind_ret_l.
+  - rewrite unfold_fmap_itree, bind_map, bind_bind; cbn. setoid_rewrite bind_ret_l.
     apply eqit_bind; reflexivity.
 Qed.
 
@@ -133,7 +133,7 @@ Proof.
   rewrite unfold_bind. (* TODO: slow *)
   rewrite (unfold_interp_state f t).
   destruct (observe t).
-  - cbn. rewrite !bind_ret_l. simpl.
+  - cbn. rewrite !bind_ret_l_. cbn.
     apply reflexivity.
   - cbn. rewrite !bind_tau, interp_state_tau.
     gstep. econstructor. gbase. apply CIH.
@@ -241,7 +241,7 @@ Lemma eutt_interp_state_loop {E F S A B C} (RS : S -> S -> Prop)
           (interp_state h (loop t2 a) s2)).
 Proof.
   intros.
-  unfold loop, bimap, Bimap_Coproduct, case_, Case_Kleisli, Function.case_sum, id_, Id_Kleisli, cat, Cat_Kleisli; cbn.
+  unfold loop, bimap, Bimap_Coproduct, case_, Case_Kleisli, Function.case_sum, inr_, Inr_Kleisli, inl_, Inl_Kleisli, lift_ktree_, id_, Id_Kleisli, cat, Cat_Kleisli; cbn.
   rewrite 2 bind_ret_l.
   eapply (eutt_interp_state_iter eq eq); auto; intros.
   rewrite 2 interp_state_bind.
@@ -249,7 +249,7 @@ Proof.
   eapply eutt_clo_bind; eauto.
   intros.
   cbn in H2; destruct (snd u1); rewrite <- (proj2 H2).
-  - rewrite bind_ret_l, 2 interp_state_ret.
+  - rewrite bind_ret_l, unfold_ret_itree, interp_state_ret.
     pstep.
     constructor.
     cbn.
